\begin{answer}
    Using Bayes we know that:
    $$
        \begin{aligned}
            p(y = 1\mid x; \phi, \mu_0, \mu_1, \Sigma) & = \frac{p(x|y=1)p(y=1)}{p(x|y=1)p(y=1) + p(x|y=0)p(y=0)}                                                                                        \\
                                                       & = \frac{1}{\frac{p(x|y=1)p(y=1)}{p(x|y=1)p(y=1)} + \frac{p(x|y=0)p(y=0)}{p(x|y=1)p(y=1)}}                                                       \\
                                                       & = \frac{1}{1+exp(-[\frac{1}{2}(x-\mu_{0})^T \Sigma^{-1} (x-\mu_{0})]+[\frac{1}{2}(x-\mu_1)^T \Sigma^{-1} (x-\mu_1)])\frac{1-\phi}{\phi}}        \\
                                                       & = \frac{1}{1+exp(-[\frac{1}{2}(x-\mu_{0})^T \Sigma^{-1} (x-\mu_{0})]+[\frac{1}{2}(x-\mu_1)^T \Sigma^{-1} (x-\mu_1) + ln(\frac{1-\phi}{\phi})])}
        \end{aligned}
    $$
    And if do some linear algebra:
    \begin{equation}
        [(x-\mu_1)^T \Sigma^{-1} (x-\mu_1)]-[(x-\mu_{0})^T \Sigma^{-1} (x-\mu_{0})]
    \end{equation}
    becomes\dots
    $$
    \begin{aligned}
        &=x^T\Sigma^{-1}x - x^T\Sigma^{-1}\mu_1 -\mu_1^T\Sigma^{-1}x +\mu_1^T\Sigma^{-1}\mu_1 - (x^T\Sigma^{-1}x - x^T\Sigma^{-1}\mu_0 -\mu_0^T\Sigma^{-1}x +\mu_0^T\Sigma^{-1}\mu_0)\\
        &= x^T\Sigma^{-1}\mu_0-x^T\Sigma^{-1}\mu_1 + \mu_0^T\Sigma^{-1}x - \mu_1^T\Sigma^{-1}x + \mu_1^T\Sigma^{-1}\mu_1 - \mu_0^T\Sigma^{-1}\mu_0\\
        &= 2(\mu_1 - \mu_0)^T\Sigma^{-1}x + \mu_0^T\Sigma^{-1}\mu_0 - \mu_1^T\Sigma^{-1}\mu_1
    \end{aligned}
    $$
    Hence:
    $$p(y = 1\mid x; \phi, \mu_0, \mu_1, \Sigma) = \frac{1}{1+exp(-[(\mu_1 - \mu_0)^T\Sigma^{-1}x + \frac{1}{2}(\mu_0^T\Sigma^{-1}\mu_0 - \mu_1^T\Sigma^{-1}\mu_1)-ln(\frac{1-\phi}{\phi})])}$$
    From that we can take $\phi$ to be $(\mu_1 - \mu_0)^T\Sigma^{-1}$ and $\phi_0$ to be $\frac{1}{2}(\mu_0^T\Sigma^{-1}\mu_0 - \mu_1^T\Sigma^{-1}\mu_1)-ln(\frac{1-\phi}{\phi})$
\end{answer}
